Cleaned up exports and begun implementing test suite calculation

FSM/fsm/Main.hs
@@ -2,9 +2,45 @@
 
 module Main where
 import FSM
+import qualified Data.List
+
 
 deriving instance Show a => Show (Set a)
 deriving instance (Show a, Show b) => Show (FSM_ext a b)
+
+showIOSequence :: [(Integer, Integer)] -> String
+showIOSequence io = "(" ++ (concat $ map show (map fst io)) ++ "/" ++  (concat $ map show (map snd io)) ++ ")"
+
+isMaximalSequence :: [(Integer, Integer)] -> [[(Integer, Integer)]] -> Bool
+isMaximalSequence seq = Prelude.all (\ seq' -> seq' == seq || (not $ Data.List.isPrefixOf seq seq'))
+
+getMaxSequences :: [[(Integer, Integer)]] -> [[(Integer, Integer)]]
+getMaxSequences seqs = Data.List.nub $ filter (\ seq -> isMaximalSequence seq seqs) seqs
+
+showTraversalTest :: ([(Integer, Integer)], [[(Integer, Integer)]]) -> String
+showTraversalTest (trav,tests) = 
+    "    Traversal sequence: " ++ (showIOSequence trav) ++ "\n" ++ 
+    "      Test sequences: " ++ (Data.List.intercalate "\n                      " $ map showIOSequence $ getMaxSequences tests) 
+
+showTest :: (Set [(Integer, Integer)], [([(Integer, Integer)], [[(Integer, Integer)]])]) -> String
+showTest (Set pr, tts) = 
+    "  Preamble:\t" ++ (Data.List.intercalate "\n      " $ map showIOSequence $ getMaxSequences pr) ++ "\n" ++ (Data.List.intercalate "\n" $ map showTraversalTest tts) 
+
+showTestSuite :: [(Set [(Integer, Integer)], [([(Integer, Integer)], [[(Integer, Integer)]])])] -> String
+showTestSuite ptts = "[\n" ++ (unlines $ map showTest ptts) ++ "]" 
+
+
+
+showTraversalTest' :: ([(Integer, Integer)], [[(Integer, Integer)]]) -> String
+showTraversalTest' (trav,tests) = 
+    "\t" ++ (showIOSequence trav) ++ "\n\t\t" ++ (Data.List.intercalate "\n\t\t" $ map showIOSequence $ getMaxSequences tests) 
+
+showTest' :: (Set [(Integer, Integer)], [([(Integer, Integer)], [[(Integer, Integer)]])]) -> String
+showTest' (Set pr, tts) = 
+    (Data.List.intercalate " " $ map showIOSequence $ getMaxSequences pr) ++ "\n" ++ (Data.List.intercalate "\n" $ map showTraversalTest' tts) 
+
+showTestSuite' :: [(Set [(Integer, Integer)], [([(Integer, Integer)], [[(Integer, Integer)]])])] -> String
+showTestSuite' ptts = "[\n" ++ (unlines $ map showTest' ptts) ++ "]" 
 
 
 main = putStrLn $ show $ maximal_repetition_sets_from_separators m_ex_DR
