FSM/Test_Suite.thy
@@ -10,6 +10,82 @@ type_synonym Test_Sequences = "IO_Sequence list"
 type_synonym Test_Case = "(Preamble_Sequence \<times> ((Traversal_Sequence \<times> Test_Sequences) list))"
 type_synonym Test_Case' = "(Preamble_Sequence set \<times> ((Traversal_Sequence \<times> Test_Sequences) list))"
 
+fun contains_io_sequence' :: "'a Transition set \<Rightarrow> 'a \<Rightarrow> IO_Sequence \<Rightarrow> bool" where
+  "contains_io_sequence' H q [] = True" |
+  "contains_io_sequence' H q (io#ios) = (\<exists> t \<in> H . t_source t = q \<and> t_input t = fst io \<and> t_output t = snd io \<and> contains_io_sequence' H (t_target t) ios)"
+
+value "contains_io_sequence' (h M_ex_H) 1 [(0,0)]"
+value "contains_io_sequence' (h M_ex_H) 1 [(0,1),(0,0)]"
+value "contains_io_sequence' (h M_ex_H) 1 [(0,1),(0,0),(0,1),(0,0),(0,1),(0,0),(0,1),(0,0)]"
+value "contains_io_sequence' (h M_ex_H) 1 [(0,1),(0,0),(0,1),(0,0),(0,1),(0,0),(0,1),(0,0),(0,0)]"
+
+
+definition contains_io_sequence :: "('a,'b) FSM_scheme \<Rightarrow> 'a \<Rightarrow> IO_Sequence \<Rightarrow> bool" where
+  "contains_io_sequence M q io = contains_io_sequence' (h M) q io"
+
+
+
+lemma contains_io_sequence_soundness :
+  assumes "q \<in> nodes M"
+  and     "contains_io_sequence M q io"
+shows "io \<in> LS M q"
+proof -
+  have "\<exists> p . path M q p \<and> p_io p = io"
+  using assms proof (induction io arbitrary: q)
+    case Nil
+    then show ?case by auto
+  next
+    case (Cons io ios)
+    then obtain t where "t \<in> h M" and "t_source t = q" and "t_input t = fst io" and "t_output t = snd io" and "contains_io_sequence M (t_target t) ios"
+      unfolding contains_io_sequence_def by auto
+   
+    obtain p where "path M (t_target t) p" and "p_io p = ios"
+      using Cons.IH[OF wf_transition_target[OF \<open>t \<in> h M\<close>] \<open>contains_io_sequence M (t_target t) ios\<close>] by blast
+  
+    have "path M q (t#p)" 
+      using \<open>path M (t_target t) p\<close> \<open>t \<in> h M\<close> \<open>t_source t = q\<close> by auto
+    moreover have "p_io (t#p) = io#ios"
+      using \<open>p_io p = ios\<close> \<open>t_input t = fst io\<close> \<open>t_output t = snd io\<close> by auto
+    ultimately show ?case
+      by auto   
+  qed
+
+  then show ?thesis by auto
+qed
+
+lemma contains_io_sequence_exhaustiveness :
+  assumes "io \<in> LS M q"
+  shows "contains_io_sequence M q io"
+proof -
+  from assms obtain p where "length p = length io" and  "path M q p" and "p_io p = io"
+    by auto
+  then show ?thesis
+  proof (induction p io arbitrary: q rule: list_induct2)
+    case Nil
+    then show ?case 
+      unfolding contains_io_sequence_def using contains_io_sequence'.simps(1) by auto
+  next
+    case (Cons t p io ios)
+    then have "path M (t_target t) p" and "p_io p = ios" 
+      by auto
+      
+    then have "contains_io_sequence M (t_target t) ios" 
+      using Cons.IH by auto
+    moreover have "t \<in> h M" and "t_source t = q" and "t_input t = fst io" and "t_output t = snd io"
+      using Cons by auto
+    ultimately have "t \<in> h M" and "t_source t = q \<and> t_input t = fst io \<and> t_output t = snd io \<and> contains_io_sequence' (h M) (t_target t) ios"
+      unfolding contains_io_sequence_def using Cons by auto
+      
+    then show ?case 
+      unfolding contains_io_sequence_def contains_io_sequence'.simps by blast
+  qed
+qed
+
+  
+
+(* TODO: only apply fail sequences? state_separation_fail_sequence_set_from_state_separator *)
+(* TODO: implement faster state_separation_fail_sequence_set_from_state_separator using the above function instead of calculating L M *)
+
 (* after each traversal sequence all state separators that r-d the reached state from some other state are added *)
 (* TODO: add only relevant separators *)
 fun test_suite_naive :: "('a,'b) FSM_scheme \<Rightarrow> nat \<Rightarrow> Test_Case' list" where
@@ -20,7 +96,7 @@ fun test_suite_naive :: "('a,'b) FSM_scheme \<Rightarrow> nat \<Rightarrow> Test
                                               (\<lambda> t . (p_io t, concat (map 
                                                           (\<lambda> qqS . LS_acyclic_opt (snd qqS))
                                                           (filter 
-                                                                  (\<lambda> qqS . fst (fst qqS) = fst qp)                                                        
+                                                                  (\<lambda> qqS . fst (fst qqS) = target t (fst qp))
                                                                   qqSS))))
                                               (m_traversal_paths M (fst qp) MRS m))) 
                                     (d_reachable_states_with_preambles M) 
