FSM/CodeExport.thy
@@ -1,14 +1,18 @@
 theory CodeExport
-imports R_Distinguishability Helper_Algorithms
+imports Test_Suite
 begin 
 
 export_code set
-	    FSM_ext
+            nat (* TODO: how to automatically export constructors?*)
+      	    FSM_ext
             r_distinguishable_state_pairs_with_separators_naive
             maximal_pairwise_r_distinguishable_state_sets_from_separators
             d_reachable_states_with_preambles
             maximal_repetition_sets_from_separators
+            test_suite_naive
             M_ex_DR
+            M_ex_H
+            M_ex_9
   in Haskell module_name FSM file_prefix fsm
 
 
